Switched to Module representation.

Game.v
@@ -1,25 +1,78 @@
 
-Structure Game :=
-{
-  player : Set;  (* The players *)
-  state : Set;   (* What the board looks like *)
-  start : state;  (* How to set it up for a new game *)
+
+Module Type Game.
+  Parameter player : Set.   (* The players *)
+  Parameter state : Set.    (* What the board looks like *)
+  Parameter start : state.  (* How to set it up for a new game *)
   
   (* The set of information potentially available to a player *)
-  observable : player -> Set;
+  Parameter observable : player -> Set.
   
   (* For each state, all the information available to a player at that state *)
-  get_observable : state -> forall p : player, observable p;
+  Parameter get_observable : state -> forall p : player, observable p.
   
   (* At each state of the game, each player has to make a decision depending *)
   (* on what he can observe of that state *)
-  decision : forall p : player, observable p -> Set;
+  Parameter decision : forall p : player, observable p -> Set.
   
   (* The rules decide the next state of the game from the decisions of *)
   (* all players decisions *)
-  rules : forall s : state,
-          (forall p:player, decision p (get_observable s p)) ->
-            state;
-}.
+  Parameter rules : forall s : state,
+    (forall p:player, decision p (get_observable s p)) ->
+    state.
+End Game.  
+
+Module BasicProperties (G : Game).
+  Import G.
+
+  Definition player_decision_space (s:state) (p:player) : Set :=
+    decision p (get_observable s p).
+    
+  Definition decision_space (s:state) : Set :=
+    forall (p:player), player_decision_space s p.
+  
+  Definition strategy (p:player) : Set :=
+    forall (h:list (observable p)) (o:observable p), decision p o.
+  
+  Definition memoryless (p:player) (s:strategy p) : Prop :=
+    exists (f:(forall (o:observable p), decision p o)),
+    forall (h:list (observable p)), s h = f.
+  
+  Definition looping_state (s:state) : Prop :=
+    forall (dec : decision_space s), rules s dec = s.
+  
+  Definition decisionless_state_player (s:state) (p:player) : Prop :=
+    not (inhabited (player_decision_space s p)).
+  
+  Definition decisionless_state (s:state) : Prop :=
+    not (inhabited (decision_space s)).
+
+  Lemma decisionless_is_looping :
+    forall s:state, decisionless_state s -> looping_state s.
+  Proof.
+    unfold decisionless_state. intros.
+    unfold looping_state. intros.
+    destruct H.
+    exact (inhabits dec).
+    Qed.
+  
+    
+End BasicProperties.
+
+
+
+Module Type WinnableGame (Import G : Game).
+  Module BP := BasicProperties G.
+  Import BP.
+  Parameter 
+
+Module Type CompleteInformationGame (Import G : Game).
+  Parameter deduce_state : forall (p:player), observable p -> state.
+  (* Function allowing each player to infer the state from observable. *)
+  
+  Axiom deduce_is_inv_obs : forall (p:player) (s:state), deduce_state p (get_observable s p) = s.
+  (* Proof that the state inferred is always correct. *)
+  
+End CompleteInformationGame.
 
 
